src/CompilationUnit.v
@@ -16,24 +16,25 @@ Definition singleton {ty} (e : expr [] ty) (name : string) : compilation_unit :=
 
 (* Initial state stuff for SourceLang *)
 
-Inductive initial_state (cu : compilation_unit) : forall tys ty, expr tys ty -> Prop := 
-| initial_intro :
+(* Not sure how to write all the dependent types for this *)
+Inductive is_callstate (cu : compilation_unit) : forall tys ty, expr tys ty -> expr tys ty -> expr tys ty -> Prop := .
+(* | initial_intro :
     forall ty expr (m : member ty (types cu)),
       hget (exprs cu) m = expr ->
-      initial_state cu nil ty expr.
+      initial_state cu nil ty expr.*)
 
 
-Inductive final_state (cu : compilation_unit) : forall tys ty, expr tys ty -> Prop :=
+Inductive final_state (cu : compilation_unit) : forall tys ty, expr tys ty -> expr tys ty -> Prop :=
 | final_intr :
     forall ty expr,
       SourceLang.value expr ->
-      final_state cu nil ty expr.
+      final_state cu nil ty expr expr.
       
-
 Definition source_semantics {ty : type} (cu : compilation_unit) : Semantics.semantics :=
   @Semantics.Semantics_gen (@SourceLang.expr nil ty) unit
+                           (@SourceLang.expr nil ty)
+                           (is_callstate cu nil ty)
                            (fun _ => @SourceLang.step nil ty)
-                           (initial_state cu nil ty)
                            (final_state cu nil ty)
                            (tt).
 
