src/SelfCloseComp.v
@@ -280,7 +280,10 @@ Section Preservation.
   Proof.
     eapply Semantics.forward_simulation_plus with (match_states := I).
     - inversion 1. (* TODO - replace with callstate matching *)
-    - intros0 II Afinal. invc Afinal. invc II. constructor. eauto using I_expr_value.
+    - intros0 II Afinal. invc Afinal. invc II.
+      eexists; split.
+      constructor. eauto using I_expr_value.
+      reflexivity.
     - intros0 Astep. intros0 II.
       eapply splus_semantics_sim, I_sim; eauto.
       destruct prog, tprog. unfold compile_cu in *. inject_pair. auto.
